tests/lean/Avl/Tree.lean
@@ -1,162 +1,44 @@
 import Avl.Funs
 import Avl.Types
 
-namespace Tree
-open avl
+namespace avl
 
 variable {T: Type}
 
--- Otherwise, Lean cannot prove termination by itself.
-@[reducible]
-def AVLTree (U: Type) := Option (AVLNode U)
-def AVLTree.nil: AVLTree T := none
-
-def AVLTree.val (t: AVLTree T): Option T := match t with
-| none => none
-| some (AVLNode.mk x _ _ _) => some x
-
-@[simp]
-lemma AVLTree.val_of_mk {x: T} {left right: AVLTree T}: AVLTree.val (AVLNode.mk x left right h) = .some x := rfl
-
-def AVLTree.left (t: AVLTree T): AVLTree T := match t with
-| none => none
-| some (AVLNode.mk _ left _ _) => left
-
-@[simp]
-lemma AVLTree.left_of_mk {x: T} {left right: AVLTree T}: AVLTree.left (AVLNode.mk x left right h) = left := rfl
-
-def AVLTree.right (t: AVLTree T): AVLTree T := match t with
-| none => none
-| some (AVLNode.mk _ _ right _) => right
-
-@[simp]
-lemma AVLTree.right_of_mk {x: T} {left right: AVLTree T}: AVLTree.right (AVLNode.mk x left right h) = right := rfl
-
-def AVLTree.memoized_height (t: AVLTree T): Primitives.Scalar .Usize := match t with
-| none => 0#usize
-| some (AVLNode.mk _ _ _ h) => h
-
-def AVLNode.left (t: AVLNode T): AVLTree T := match t with
-| AVLNode.mk _ left _ _ => left
-
-@[simp]
-lemma AVLTree.left_of_some {t: AVLNode T}: AVLTree.left (some t) = AVLNode.left t := by cases t; simp [AVLNode.left]
-
-@[simp]
-lemma AVLNode.left_of_mk {x: T} {left right: AVLTree T}: AVLNode.left (AVLNode.mk x left right h) = left := rfl
-
-def AVLNode.right (t: AVLNode T): AVLTree T := match t with
-| AVLNode.mk _ _ right _ => right
-
-@[simp]
-lemma AVLTree.right_of_some {t: AVLNode T}: AVLTree.right (some t) = AVLNode.right t := by cases t; simp [AVLNode.right]
-
-@[simp]
-lemma AVLNode.right_of_mk {x: T} {left right: AVLTree T}: AVLNode.right (AVLNode.mk x left right h) = right := rfl
-
-def AVLNode.val (t: AVLNode T): T := match t with
-| AVLNode.mk x _ _ _ => x
-
-@[simp]
-lemma AVLNode.val_of_mk {x: T} {left right: AVLTree T}: AVLNode.val (AVLNode.mk x left right h) = x := rfl
-
-def AVLNode.memoized_height (t: AVLNode T): Primitives.Scalar .Usize := match t with
-| AVLNode.mk _ _ _ h => h
+abbrev Child T := Option (Node T)
 
 -- TODO: rename to node_height
 mutual
-def AVLTree.height_node: AVLNode T -> Nat
-| AVLNode.mk y left right _ => 1 + max (AVLTree.height left) (AVLTree.height right)
+@[simp]
+def Node.compute_height: Node T -> Nat
+| Node.mk y left right _ => 1 + max (Child.compute_height left) (Child.compute_height right)
 
-def AVLTree.height: AVLTree T -> Nat
+@[simp]
+def Child.compute_height: Child T -> Nat
 | none => 0
-| some n => AVLTree.height_node n
+| some n => 1 + Node.compute_height n
 end
 
-@[simp]
-def AVLTree.height_of_none: @AVLTree.height T none = 0 := by simp [AVLTree.height]
-
-@[simp]
-def AVLTree.height_of_some {t: AVLNode T}: AVLTree.height (some t) = AVLTree.height_node t := by simp [AVLTree.height]
-
-@[simp]
-def AVLTree.height_node_of_mk {left right: AVLTree T}: AVLTree.height_node (AVLNode.mk x left right h) = 1 + max (AVLTree.height left) (AVLTree.height right) := by simp [AVLTree.height_node]
-
-def AVLTree.height_node_eq (t: AVLNode T): AVLTree.height_node t = 1 + max (AVLTree.height (AVLNode.left t)) (AVLTree.height (AVLNode.right t)) := by sorry
-
-def AVLNode.height_left_lt_tree (left: AVLNode T) {right: AVLTree T}: AVLTree.height_node left < AVLTree.height_node (AVLNode.mk x (some left) right h) := by
-  simp only [AVLTree.height_node_of_mk, AVLTree.height_of_some]
-  rw [Nat.add_comm, Nat.add_one]
-  exact Nat.lt_succ_of_le (le_max_left _ _)
-
-def AVLNode.height_right_lt_tree (right: AVLNode T) {left: AVLTree T}: AVLTree.height_node right < AVLTree.height_node (AVLNode.mk x left (some right) h) := by
-  simp only [AVLTree.height_node_of_mk, AVLTree.height_of_some]
-  rw [Nat.add_comm, Nat.add_one]
-  exact Nat.lt_succ_of_le (le_max_right _ _)
-
-def AVLTree.height_left_lt_tree (left right: AVLTree T): AVLTree.height left < AVLTree.height (some (AVLNode.mk x left right h)) := by
-  match left with
-  | none => simp [height, height_node]
-  | some left => simp only [height, AVLNode.height_left_lt_tree left]
-
-def AVLTree.height_left_lt_tree' (t: AVLNode T): AVLTree.height (AVLNode.left t) < AVLTree.height (some t) := by
-  match t with
-  | AVLNode.mk _ left right h => simp only [AVLNode.left, AVLTree.height_left_lt_tree]
-
-def AVLTree.height_left_le_tree' (t: AVLTree T): AVLTree.height (AVLTree.left t) ≤ AVLTree.height t := by
-  match t with
-  | none => simp [height, left]
-  | some t => simp only [AVLTree.left_of_some, le_of_lt (AVLTree.height_left_lt_tree' t)]
-
-def AVLTree.height_right_lt_tree (left right: AVLTree T): AVLTree.height right < AVLTree.height (some (AVLNode.mk x left right h)) := by
-  match right with
-  | none => simp [height, height_node]
-  | some right => simp only [height, AVLNode.height_right_lt_tree right]
-
-def AVLTree.height_right_lt_tree' (t: AVLNode T): AVLTree.height (AVLNode.right t) < AVLTree.height (some t) := by
-  match t with
-  | AVLNode.mk _ left right h => simp only [AVLNode.right, AVLTree.height_right_lt_tree]
-
-
-def AVLTreeSet.nil: AVLTreeSet T := { root := AVLTree.nil }
+def Tree.nil: Tree T := { root := none }
 
 -- Automatic synthesization of this seems possible at the Lean level?
-instance: Inhabited (AVLTree T) where
-  default := AVLTree.nil
+instance: Inhabited (Tree T) where
+  default := Tree.nil
 
-instance: Inhabited (AVLTreeSet T) where
-  default := AVLTreeSet.nil
+instance [Inhabited T]: Inhabited (Node T) where
+  default := ⟨ Inhabited.default, none, none, 0#usize ⟩
 
-instance: Coe (Option (AVLNode T)) (AVLTree T) where
-  coe x := x
-
--- TODO: ideally, it would be nice if we could generalize
--- this to any `BinaryTree` typeclass.
-
-def AVLTree.mem (tree: AVLTree T) (x: T) :=
+mutual
+@[simp] def Child.v (tree: Child T) : Set T :=
   match tree with
-  | none => False
-  | some (AVLNode.mk y left right _) => x = y ∨ AVLTree.mem left x ∨ AVLTree.mem right x
+  | none => ∅
+  | some node => node.v
 
-#check Function.funext_iff
-@[simp]
-def AVLTree.mem_none: AVLTree.mem none = ({}: Set T) := by
-  rw [Function.funext_iff]
-  simp [mem, EmptyCollection.emptyCollection]
+@[simp] def Node.v (node : Node T) : Set T :=
+  match node with
+  | .mk x left right _ => {x} ∪ Child.v left ∪ Child.v right
+end
 
-@[simp]
-def AVLTree.mem_some {x: T} {left right: AVLTree T}: AVLTree.mem (some (AVLNode.mk x left right h)) = (({x}: Set T) ∪ AVLTree.mem left ∪ AVLTree.mem right) := by
-  ext y
-  rw [AVLTree.mem]
-  simp [Set.insert_union]
-  simp [Set.insert_def, Set.setOf_set, Set.mem_def, Set.union_def]
+def Tree.v (t: Tree T): Set T := Child.v t.root
 
--- TODO(reinforcement): ∪ is actually disjoint if we prove this is a binary search tree.
-
-def AVLTree.set (t: AVLTree T): Set T := _root_.setOf (AVLTree.mem t)
-
-@[simp]
-def AVLTree.set_some {x: T} {left right: AVLTree T}: AVLTree.set (some (AVLNode.mk x left right h)) = {x} ∪ AVLTree.set left ∪ AVLTree.set right := by
-  simp [set, setOf]
-
-end Tree
+end avl
