tests/lean/Avl/Spec.lean
@@ -1,0 +1,143 @@
+import Avl.Tree
+
+namespace avl
+
+open Primitives (Result Scalar)
+open avl Node Ordering Tree
+
+mutual
+@[simp] def Child.forall (p: Node T -> Prop) (child : Child T) : Prop :=
+  match child with
+  | none => true
+  | some child => child.forall p
+termination_by Child.compute_height child
+decreasing_by simp_wf
+
+def Node.forall (p: Node T -> Prop) (node : Node T) : Prop :=
+  p node ∧
+  Child.forall p node.left ∧ Child.forall p node.right
+termination_by Node.compute_height node
+decreasing_by all_goals (simp_wf <;> split <;> simp <;> scalar_tac)
+end
+
+@[simp]
+theorem Child.forall_left {p: Node T -> Prop} {t: Node T}: Node.forall p t -> Child.forall p t.left := by
+  cases t; simp_all [Node.forall]
+
+@[simp]
+theorem Child.forall_right {p: Node T -> Prop} {t: Node T}: Child.forall p t -> Child.forall p t.right := by
+  cases t; simp_all [Node.forall]
+
+/-
+theorem Child.forall_not_mem {a: T} (p: Node T -> Prop) (t: Child T): ¬ p a -> Child.forall p t -> a ∉ Child.v t
+  := fun Hnpa Hpt => by
+  cases t <;> simp
+  unfold Child.forall Node.forall at Hpt
+  split at Hpt; simp_all
+  split_conjs
+  . by_contra hab; rw [hab] at Hnpa; simp_all
+  . apply (forall_not_mem p) <;> simp [*]
+  . apply (forall_not_mem p) <;> simp [*]
+
+theorem Child.forall_not_mem' {a: T} (p: T -> Prop) (t: Option (Node T)):
+  p a -> Child.forall (fun x =>  ¬p x) t -> a ∉ Child.v t
+  := by
+  intro Hpa Hnpt
+  refine' Child.forall_not_mem (fun x => ¬ p x) t _ _
+  simp [Hpa]
+  exact Hnpt
+-/
+
+mutual
+theorem Child.forall_imp {p q: Node T -> Prop} {t: Child T}: (∀ x, p x -> q x) -> Child.forall p t -> Child.forall q t
+  := by
+  match t with
+  | none => simp
+  | some node =>
+    simp
+    intros
+    apply @Node.forall_imp T p q <;> tauto
+
+theorem Node.forall_imp {p q: Node T -> Prop} {t: Node T}: (∀ x, p x -> q x) -> Node.forall p t -> Node.forall q t := by
+  match t with
+  | .mk x left right height =>
+    simp [Node.forall]
+    intros Himp Hleft Hright Hx
+    simp [*]
+    split_conjs <;> apply @Child.forall_imp T p q <;> tauto
+
+end
+
+def Node.balancingFactor (node : Node T) : ℤ :=
+  Child.compute_height node.left - Child.compute_height node.right
+
+def Child.balancingFactor (t: Child T): ℤ :=
+  match t with
+  | .none => 0
+  | .some x => x.balancingFactor
+
+variable [LinearOrder T]
+
+def Node.inv_aux (node : Node T) : Prop :=
+  node.height.val = node.compute_height ∧
+  Child.forall (fun node' => node'.value < node.value) node.left ∧
+  Child.forall (fun node' => node.value < node'.value) node.right ∧
+  -1 ≤ node.balancingFactor ∧ node.balancingFactor ≤ 1
+
+def Node.inv (node : Node T) : Prop :=
+  Node.forall Node.inv_aux node
+
+@[simp]
+def Child.inv (child : Child T) : Prop :=
+  match child with
+  | none => true
+  | some node => node.inv
+
+@[simp]
+theorem Node.inv_left {t: Node T}: t.inv -> Child.inv t.left := by
+  simp [Node.inv]
+  intro
+  cases t; simp
+  split <;> try simp_all [Node.forall]
+
+@[simp]
+theorem Node.inv_right {t: Node T}: t.inv -> Child.inv t.right := by
+  simp [Node.inv]
+  intro
+  cases t; simp
+  split <;> try simp_all [Node.forall]
+
+/-
+-- TODO: ask at most for LT + Irreflexive (lt_irrefl) + Trichotomy (le_of_not_lt)?
+theorem left_pos {left right: Option (Node T)} {a x: T}: BST.Invariant (some (Node.mk a left right h)) -> x ∈ Tree.set (Node.mk a left right h) -> x < a -> x ∈ Tree.set left := fun Hbst Hmem Hxa => by
+   simp [Tree.set_some] at Hmem
+   rcases Hmem with (Heq | Hleft) | Hright
+   . rewrite [Heq] at Hxa; exact absurd Hxa (lt_irrefl _)
+   . assumption
+   . exfalso
+
+     -- Hbst -> x ∈ right -> ForallNode (fun v => ¬ v < a)
+     refine' ForallNode.not_mem' (fun v => v < a) right Hxa _ _
+     simp [le_of_not_lt]
+     cases Hbst with
+     | some _ _ _ _ Hforall _ =>
+       refine' ForallNode.imp _ Hforall
+       exact fun x => le_of_lt
+     assumption
+
+theorem right_pos {left right: Option (Node T)} {a x: T}: BST.Invariant (some (Node.mk a left right h)) -> x ∈ Tree.set (Node.mk a left right h) -> a < x -> x ∈ Tree.set right := fun Hbst Hmem Hax => by
+   simp [Tree.set_some] at Hmem
+   rcases Hmem with (Heq | Hleft) | Hright
+   . rewrite [Heq] at Hax; exact absurd Hax (lt_irrefl _)
+   . exfalso
+     refine' ForallNode.not_mem' (fun v => a < v) left Hax _ _
+     simp [le_of_not_lt]
+     cases Hbst with
+     | some _ _ _ Hforall _ _ =>
+       refine' ForallNode.imp _ Hforall
+       exact fun x => le_of_lt
+     assumption
+   . assumption
+-/
+
+end avl
